vir file cleanup

theories/vir/contextual.v
@@ -2,8 +2,8 @@ From iris.prelude Require Import options.
 
 From velliris.logic Require Import satisfiable.
 From velliris.program_logic Require Import program_logic.
-From velliris.vir Require Import
-  vir val_rel heapbij adequacy spec globalbij logical_relations fundamental
+From velliris.vir Require Import vir val_rel
+  heapbij adequacy spec globalbij logical_relations fundamental
   contextual_mcfg.
 
 From Vellvm Require Import Syntax.DynamicTypes Handlers Syntax.LLVMAst
@@ -15,21 +15,54 @@ Import LLVMEvents.
 
 Set Default Proof Using "Type*".
 
+(** *Initial state *)
+
+Definition empty_vir_state : vir_state :=
+  (∅, (nil, nil), (∅, ∅, Mem.Singleton nil)).
+
+(* Returns `true` only if both function are named and have
+     the same name. *)
+Definition function_name_eq (a b:function_id) : bool :=
+  match a, b with
+  | Name aname, Name bname => String.eqb aname bname
+  | _, _ => false
+  end.
+
+(* Initial state: all function declaration names are allocated in global
+   environment, and otherwise the state is empty *)
+Definition allocate_declaration_prog (d:declaration dtyp) (σ : vir_state) : vir_state :=
+  match List.find (fun x => function_name_eq (dc_name d) (dc_name x))
+          IntrinsicsDefinitions.defined_intrinsics_decls with
+  | Some _ => σ
+  | None =>
+      let '(g, l, (m, v)) :=
+        fmap_mem (vir.allocate_non_void DTYPE_Pointer) σ
+      in
+      let g :=
+        global_write (dc_name d) (DVALUE_Addr v) g
+      in
+      (g, l, m)
+  end.
+
+Definition allocate_declarations_prog
+  (ds:list (declaration dtyp)) (σ : vir_state) : vir_state :=
+  List.fold_left (fun acc x => allocate_declaration_prog x acc) ds σ.
+
+Definition init_state ds := allocate_declarations_prog ds empty_vir_state.
+
 (** *Whole-program refinement *)
 Section prog_ref.
 
-  (* Initial relation on states *)
-  Context (I : vir_state -> vir_state -> Prop).
+  Context (ds : list (declaration dtyp)).
 
   (* If the initial states are related by some relation, and the expressions
      are well formed (i.e. the source program does not "go wrong" and the
      expressions are closed after denotation), then the resulting programs
      are observationally equivalent to each other using [eutt]. *)
   Definition prog_ref (e_t e_s : expr vir_lang uvalue) :=
-    ∀ σ_t σ_s,
-      I σ_t σ_s ->
-      well_formed (⟦ e_t ⟧ σ_t) (⟦ e_s ⟧ σ_s) ->
-      eutt obs_val_res (⟦ e_t ⟧ σ_t) (⟦ e_s ⟧ σ_s).
+    let σ := init_state ds in
+    well_formed (⟦ e_t ⟧ σ) (⟦ e_s ⟧ σ) ->
+    eutt obs_val_res (⟦ e_t ⟧ σ) (⟦ e_s ⟧ σ).
 
 End prog_ref.
 
@@ -53,13 +86,6 @@ Definition ctx_wf (C : context) :=
      consequence of the fundamental theorem. *)
   Forall (fun x => dc_attrs x = nil) (CFG.m_declarations C)
 .
-(* Generating a well-formed global out of the definitions in a context *)
-Definition init_global (names : list function_id) :=
-  snd (List.fold_left
-    (fun '(acc, g) id =>
-      (S acc,
-        <[ id := DVALUE_Addr (Z.of_nat acc, 0%Z) ]> g)) names
-          (0%nat, (∅ : vir.globals))).
 
 
 (** *Top-level Contextual Refinement *)
@@ -87,7 +113,8 @@ Section CR_definition.
     (2) restating the denotation of mutually-recursive control flow graps using
         [denote_mcfg]. *)
   Definition fill_ctx (C : context) e :=
-    denote_vellvm_main (fill_mcfg_defs C e).
+    Monad.bind (mcfg_definitions (fill_mcfg_defs C e))
+        (fun defs => denote_mcfg defs ret_typ (DVALUE_Addr main) args).
 
   (* Contextual refinement. *)
   Definition ctx_ref e_t e_s: Prop :=
@@ -97,84 +124,84 @@ Section CR_definition.
       (* The names of the declarations are the same *)
       dc_name (df_prototype e_t.2) = dc_name (df_prototype e_s.2) ->
       (* Implies whole-program refinement *)
-      prog_ref I (fill_ctx C e_t) (fill_ctx C e_s).
+      prog_ref (m_declarations C) (fill_ctx C e_t) (fill_ctx C e_s).
 
 End CR_definition.
 
-(* Initial relation on states; there is a [main] and [null] address in the
-    state.
-  The memory and frame is empty except for the main and null address. *)
-Definition init_state (main : Addr.addr) (fun_names : list function_id) : vir_state -> Prop :=
-  fun '(g, (l, ls), (m, f)) =>
-    (* The global environment contains the names of function declarations in
-        the context [C]. *)
-      g = init_global (fun_names)
-    (* The local environment and local stack is empty *)
-    /\ l = nil /\ ls = nil
-    (* The memory has [main] and [null] allocated *)
-    /\ m = ({[ main.1 := dvalue_to_block DVALUE_None;
-              Addr.null.1 := dvalue_to_block DVALUE_None ]},
-            {[ main.1; Addr.null.1 ]})
-    (* The frame has the main and null address *)
-    /\ f = Mem.Singleton [ main.1; Addr.null.1 ].
+(* (* Initial relation on states; there is a [main] and [null] address in the *)
+(*     state. *)
+(*   The memory and frame is empty except for the main and null address. *) *)
+(* Definition init_state (main : Addr.addr) (fun_names : list function_id) : vir_state -> Prop := *)
+(*   fun '(g, (l, ls), (m, f)) => *)
+(*     (* The global environment contains the names of function declarations in *)
+(*         the context [C]. *) *)
+(*       g = init_global (fun_names) *)
+(*     (* The local environment and local stack is empty *) *)
+(*     /\ l = nil /\ ls = nil *)
+(*     (* The memory has [main] and [null] allocated *) *)
+(*     /\ m = ({[ main.1 := dvalue_to_block DVALUE_None; *)
+(*               Addr.null.1 := dvalue_to_block DVALUE_None ]}, *)
+(*             {[ main.1; Addr.null.1 ]}) *)
+(*     (* The frame has the main and null address *) *)
+(*     /\ f = Mem.Singleton [ main.1; Addr.null.1 ]. *)
 
-(* The relational variant, with the added condition that the [main] and [null]
-  addresses are not equivalent to each other. *)
-Definition init_state_rel (main : Addr.addr) C : vir_state -> vir_state -> Prop :=
-  fun σ_t σ_s =>
-    main.1 <> Addr.null.1 /\
-    init_state main C σ_t /\ init_state main C σ_s.
+(* (* The relational variant, with the added condition that the [main] and [null] *)
+(*   addresses are not equivalent to each other. *) *)
+(* Definition init_state_rel (main : Addr.addr) C : vir_state -> vir_state -> Prop := *)
+(*   fun σ_t σ_s => *)
+(*     main.1 <> Addr.null.1 /\ (* Do we say something about the rest of the state? *) *)
+(*     init_state main C σ_t /\ init_state main C σ_s. *)
 
-Section CR_properties.
+(* Section CR_properties. *)
 
-  Context {Σ} `{!sheapGS Σ, !checkedoutGS Σ, !heapbijGS Σ}.
-  Context (ret_typ : dtyp) (main : Addr.addr) (args : list uvalue).
+(*   Context {Σ} `{!sheapGS Σ, !checkedoutGS Σ, !heapbijGS Σ}. *)
+(*   Context (ret_typ : dtyp) (main : Addr.addr) (args : list uvalue). *)
 
-  (* TODO *)
-  Lemma contains_keys_init_global names :
-    contains_keys (init_global names) names.
-  Proof.
-    induction names; cbn; eauto; first set_solver.
-    rewrite /contains_keys. cbn. rewrite /init_global; cbn.
-  Admitted.
+(*   (* (* TODO *) *) *)
+(*   (* Lemma contains_keys_init_global names : *) *)
+(*   (*   contains_keys (init_global names) names. *) *)
+(*   (* Proof. *) *)
+(*   (*   induction names; cbn; eauto; first set_solver. *) *)
+(*   (*   rewrite /contains_keys. cbn. rewrite /init_global; cbn. *) *)
+(*   (* Admitted. *) *)
 
-  (* TODO *)
-  Lemma nodup_codomain_init_global names :
-    NoDup_codomain (filter_keys (init_global names) names).
-  Proof. Admitted.
+(*   (* (* TODO *) *) *)
+(*   (* Lemma nodup_codomain_init_global names : *) *)
+(*   (*   NoDup_codomain (filter_keys (init_global names) names). *) *)
+(*   (* Proof. Admitted. *) *)
 
-  Lemma ctx_wf_implies_CFG_WF C :
-   ctx_wf C ->
-   CFG_WF C (init_global (CFG_names C)) (init_global (CFG_names C)).
-  Proof.
-    intros (?&?&?&?).
-    repeat (split; eauto);
-      eauto using contains_keys_init_global, nodup_codomain_init_global.
-  Qed.
+(*   Lemma ctx_wf_implies_CFG_WF C : *)
+(*    ctx_wf C -> *)
+(*    CFG_WF C (init_global (CFG_names C)) (init_global (CFG_names C)). *)
+(*   Proof. *)
+(*     intros (?&?&?&?). *)
+(*     repeat (split; eauto); *)
+(*       eauto using contains_keys_init_global, nodup_codomain_init_global. *)
+(*   Qed. *)
 
-  Lemma ctx_wf_fill_mcfg_defs C decl e_t:
-    ctx_wf (fill_mcfg_defs C (decl, e_t)) ->
-    ctx_wf C.
-  Proof.
-    rewrite /ctx_wf.
-    intros. destructb.
-    cbn in *. split; eauto. nodup.
-    apply Forall_cons in H1, H2.
-    destructb.
-    repeat split; eauto.
-  Qed.
+(*   Lemma ctx_wf_fill_mcfg_defs C decl e_t: *)
+(*     ctx_wf (fill_mcfg_defs C (decl, e_t)) -> *)
+(*     ctx_wf C. *)
+(*   Proof. *)
+(*     rewrite /ctx_wf. *)
+(*     intros. destructb. *)
+(*     cbn in *. split; eauto. nodup. *)
+(*     apply Forall_cons in H1, H2. *)
+(*     destructb. *)
+(*     repeat split; eauto. *)
+(*   Qed. *)
 
-  Lemma ctx_wf_hole_attr C decl e_t:
-    ctx_wf (fill_mcfg_defs C (decl, e_t)) ->
-    (dc_attrs decl = nil).
-  Proof.
-    rewrite /ctx_wf.
-    intros. destructb.
-    clear -H2. cbn in *.
-    apply Forall_cons in H2; by destructb.
-  Qed.
+(*   Lemma ctx_wf_hole_attr C decl e_t: *)
+(*     ctx_wf (fill_mcfg_defs C (decl, e_t)) -> *)
+(*     (dc_attrs decl = nil). *)
+(*   Proof. *)
+(*     rewrite /ctx_wf. *)
+(*     intros. destructb. *)
+(*     clear -H2. cbn in *. *)
+(*     apply Forall_cons in H2; by destructb. *)
+(*   Qed. *)
 
-End CR_properties.
+(* End CR_properties. *)
 
 (* Well-formedness on globals: all global values are self-related *)
 Definition globals_WF `{heapbijGS Σ} (g : vir.globals) : iPropI Σ :=
@@ -186,133 +213,133 @@ Definition init_keys (main : Addr.addr) : list global_id :=
 (* We can instantiate a state interpretation with corresponding ghost resources
   on states that satisfy the initializaition relation [I] *)
 (* IY : Is there a cleaner way to state this lemma? *)
-Lemma initialize_state_interp `{sheapGpreS Σ} `{heapbijGpreS Σ} `{checkedoutGpreS Σ} :
-  forall main σ_t σ_s e_t e_s,
-    let init_keys := init_keys main in
-    let g := init_global init_keys in
-    init_state_rel main init_keys σ_t σ_s ->
+Lemma initialize_state_interp ds `{sheapGpreS Σ} `{heapbijGpreS Σ} `{checkedoutGpreS Σ} :
+  forall e_t e_s,
+    (* let init_keys := init_keys main in *)
     (∀ `(sheapGS Σ, checkedoutGS Σ, heapbijGS Σ),
-        globals_WF g ∗ <pers> fun_logrel e_t e_s ∅) ==∗
+        <pers> fun_logrel e_t e_s ∅) ==∗
     ∃ (H_sh : sheapGS Σ) (H_bij : heapbijGS Σ) (H_c : checkedoutGS Σ),
-      state_interp σ_t σ_s ∗
-      target_globals g ∗ source_globals g ∗
+      state_interp (init_state ds) (init_state ds) ∗
+      target_globals (init_state ds).1 ∗
+      source_globals (init_state ds).1 ∗
     ∃ γ_t γ_s,
         checkout ∅ ∗ stack_tgt [γ_t] ∗ stack_src [γ_s].
 Proof.
   rename H into H_shp, H0 into H_bijp, H1 into H_cp.
-  intros * HI.
+(*   intros * HI. *)
 
-  iMod (@sheap_init Σ _ g g) as (Hsh) "(Hh_t & Hh_s & H)".
-  iMod (@heapbij_init Σ _ _ ∅) as (Hhb) "Hbij".
-  iMod (@checkedout_init Σ _ ∅) as (Hc) "[Hc1 Hc2]".
+(*   iMod (@sheap_init Σ _ g g) as (Hsh) "(Hh_t & Hh_s & H)". *)
+(*   iMod (@heapbij_init Σ _ _ ∅) as (Hhb) "Hbij". *)
+(*   iMod (@checkedout_init Σ _ ∅) as (Hc) "[Hc1 Hc2]". *)
 
-  rewrite /state_interp.
+(*   rewrite /state_interp. *)
 
-  iDestruct "H" as "(Hh_tf & Hb_t & Hg_t & Hh_sf & Hb_s & Hg_s & H)".
+(*   iDestruct "H" as "(Hh_tf & Hb_t & Hg_t & Hh_sf & Hb_s & Hg_s & H)". *)
 
-  iDestruct "H" as "(Ht & Hs)".
-  iDestruct "Ht" as (?) "(Hst_t & Hl_t & Hld_t & Ha_t)".
-  iDestruct "Hs" as (?) "(Hst_s & Hl_s & Hld_s & Ha_s)".
+(*   iDestruct "H" as "(Ht & Hs)". *)
+(*   iDestruct "Ht" as (?) "(Hst_t & Hl_t & Hld_t & Ha_t)". *)
+(*   iDestruct "Hs" as (?) "(Hst_s & Hl_s & Hld_s & Ha_s)". *)
 
-  (* Allocate null bij *)
-  destruct σ_t as ((?&?&?)&(?&?)&?).
-  destruct σ_s as ((?&?&?)&(?&?)&?).
+(*   (* Allocate null bij *) *)
+(*   destruct σ_t as ((?&?&?)&(?&?)&?). *)
+(*   destruct σ_s as ((?&?&?)&(?&?)&?). *)
 
-  destruct HI as (Hun & ?&?&?&?&?&?); subst; inv H3.
-  destruct H as (?&?&?&?&?); subst; inv H2.
+(*   destruct HI as (Hun & ?&?&?&?&?&?); subst; inv H3. *)
+(*   destruct H as (?&?&?&?&?); subst; inv H2. *)
 
-  (** *Allocate null address *)
-  (* Allocate at [Addr.null] on target side *)
-  iCombine ("Ha_t Hst_t Hh_t") as "H".
-  iPoseProof
-    (heap_ctx_alloc _ Addr.null.1
-       DVALUE_None ((∅, ∅), Singleton ∅) [γf] _ _ _ _ _ DTYPE_Void) as "Halloc_t";
-    [ set_solver | cbn; set_solver | constructor | ].
-  rewrite allocaS_eq /allocaS_def. rewrite /stack.
-  iSpecialize ("Halloc_t" with "H"). iMod "Halloc_t".
+(*   (** *Allocate null address *) *)
+(*   (* Allocate at [Addr.null] on target side *) *)
+(*   iCombine ("Ha_t Hst_t Hh_t") as "H". *)
+(*   iPoseProof *)
+(*     (heap_ctx_alloc _ Addr.null.1 *)
+(*        DVALUE_None ((∅, ∅), Singleton ∅) [γf] _ _ _ _ _ DTYPE_Void) as "Halloc_t"; *)
+(*     [ set_solver | cbn; set_solver | constructor | ]. *)
+(*   rewrite allocaS_eq /allocaS_def. rewrite /stack. *)
+(*   iSpecialize ("Halloc_t" with "H"). iMod "Halloc_t". *)
 
-  (* Allocate at [Addr.null] on source side *)
-  iCombine ("Ha_s Hst_s Hh_s") as "H".
-  iPoseProof
-    (heap_ctx_alloc _ Addr.null.1
-       DVALUE_None ((∅, ∅), Singleton ∅) [γf0] _ _ _ _ _ DTYPE_Void) as "Halloc_s";
-    [ set_solver | cbn; set_solver | constructor | ].
-  rewrite allocaS_eq /allocaS_def. rewrite /stack.
-  iSpecialize ("Halloc_s" with "H"). iMod "Halloc_s".
+(*   (* Allocate at [Addr.null] on source side *) *)
+(*   iCombine ("Ha_s Hst_s Hh_s") as "H". *)
+(*   iPoseProof *)
+(*     (heap_ctx_alloc _ Addr.null.1 *)
+(*        DVALUE_None ((∅, ∅), Singleton ∅) [γf0] _ _ _ _ _ DTYPE_Void) as "Halloc_s"; *)
+(*     [ set_solver | cbn; set_solver | constructor | ]. *)
+(*   rewrite allocaS_eq /allocaS_def. rewrite /stack. *)
+(*   iSpecialize ("Halloc_s" with "H"). iMod "Halloc_s". *)
 
-  iDestruct "Halloc_t" as "(Hh_t & %Hin_t & Ha_t & Hst_t & Hv_t & hb_t)".
-  iDestruct "Halloc_s" as "(Hh_s & %Hin_s & Ha_s & Hst_s & Hv_s & hb_s)".
+(*   iDestruct "Halloc_t" as "(Hh_t & %Hin_t & Ha_t & Hst_t & Hv_t & hb_t)". *)
+(*   iDestruct "Halloc_s" as "(Hh_s & %Hin_s & Ha_s & Hst_s & Hv_s & hb_s)". *)
 
-  (* Extend global bij *)
-  rewrite !mapsto_dval_eq /mapsto_dval_def.
-  iAssert (lb_rel (dvalue_to_block DVALUE_None) (dvalue_to_block DVALUE_None))%I as "Hb".
-  { rewrite /lb_rel. cbn.
-    rewrite /mem_byte_rel. rewrite /init_block; cbn.
-    simpl. iSplit.
-    { iIntros (???). inversion H. }
-    { done. } }
-  iDestruct (heapbij_insert with "Hbij Hv_t Hv_s Hb hb_t hb_s") as ">(Hbij & #Haddr_null)".
+(*   (* Extend global bij *) *)
+(*   rewrite !mapsto_dval_eq /mapsto_dval_def. *)
+(*   iAssert (lb_rel (dvalue_to_block DVALUE_None) (dvalue_to_block DVALUE_None))%I as "Hb". *)
+(*   { rewrite /lb_rel. cbn. *)
+(*     rewrite /mem_byte_rel. rewrite /init_block; cbn. *)
+(*     simpl. iSplit. *)
+(*     { iIntros (???). inversion H. } *)
+(*     { done. } } *)
+(*   iDestruct (heapbij_insert with "Hbij Hv_t Hv_s Hb hb_t hb_s") as ">(Hbij & #Haddr_null)". *)
 
-  (** *Allocate main address *)
-  (* Allocate at [Addr.main] on target side *)
-  iCombine ("Ha_t Hst_t Hh_t") as "H".
-  iPoseProof
-    (heap_ctx_alloc _ main.1
-       DVALUE_None (({[Addr.null.1:=dvalue_to_block DVALUE_None]}, {[Addr.null.1]})
-         , Mem.Singleton [Addr.null.1]) [γf] _ _ _ _ _ DTYPE_Void) as "Halloc_t".
-  { cbn; rewrite lookup_singleton_ne; auto. }
-  { cbn; set_solver. }
-  { constructor. }
+(*   (** *Allocate main address *) *)
+(*   (* Allocate at [Addr.main] on target side *) *)
+(*   iCombine ("Ha_t Hst_t Hh_t") as "H". *)
+(*   iPoseProof *)
+(*     (heap_ctx_alloc _ main.1 *)
+(*        DVALUE_None (({[Addr.null.1:=dvalue_to_block DVALUE_None]}, {[Addr.null.1]}) *)
+(*          , Mem.Singleton [Addr.null.1]) [γf] _ _ _ _ _ DTYPE_Void) as "Halloc_t". *)
+(*   { cbn; rewrite lookup_singleton_ne; auto. } *)
+(*   { cbn; set_solver. } *)
+(*   { constructor. } *)
 
-  rewrite allocaS_eq /allocaS_def. rewrite /stack.
-  cbn. rewrite !insert_empty !union_empty_r_L.
-  iSpecialize ("Halloc_t" with "H"). iMod "Halloc_t".
+(*   rewrite allocaS_eq /allocaS_def. rewrite /stack. *)
+(*   cbn. rewrite !insert_empty !union_empty_r_L. *)
+(*   iSpecialize ("Halloc_t" with "H"). iMod "Halloc_t". *)
 
-  (* Allocate at [Addr.main] on source side *)
-  iCombine ("Ha_s Hst_s Hh_s") as "H".
-  iPoseProof
-    (heap_ctx_alloc _ main.1
-       DVALUE_None (({[Addr.null.1:=dvalue_to_block DVALUE_None]}, {[Addr.null.1]})
-         , Mem.Singleton [Addr.null.1]) [γf0] _ _ _ _ _ DTYPE_Void) as "Halloc_s".
-  { cbn; rewrite lookup_singleton_ne; auto. }
-  { cbn; set_solver. }
-  { constructor. }
+(*   (* Allocate at [Addr.main] on source side *) *)
+(*   iCombine ("Ha_s Hst_s Hh_s") as "H". *)
+(*   iPoseProof *)
+(*     (heap_ctx_alloc _ main.1 *)
+(*        DVALUE_None (({[Addr.null.1:=dvalue_to_block DVALUE_None]}, {[Addr.null.1]}) *)
+(*          , Mem.Singleton [Addr.null.1]) [γf0] _ _ _ _ _ DTYPE_Void) as "Halloc_s". *)
+(*   { cbn; rewrite lookup_singleton_ne; auto. } *)
+(*   { cbn; set_solver. } *)
+(*   { constructor. } *)
 
-  rewrite allocaS_eq /allocaS_def. rewrite /stack.
-  iSpecialize ("Halloc_s" with "H"). iMod "Halloc_s".
+(*   rewrite allocaS_eq /allocaS_def. rewrite /stack. *)
+(*   iSpecialize ("Halloc_s" with "H"). iMod "Halloc_s". *)
 
-  iDestruct "Halloc_t" as "(Hh_t & %Hin_t' & Ha_t & Hs_t & Hv_t & hb_t)".
-  iDestruct "Halloc_s" as "(Hh_s & %Hin_s' & Ha_s & Hs_s & Hv_s & hb_s)".
+(*   iDestruct "Halloc_t" as "(Hh_t & %Hin_t' & Ha_t & Hs_t & Hv_t & hb_t)". *)
+(*   iDestruct "Halloc_s" as "(Hh_s & %Hin_s' & Ha_s & Hs_s & Hv_s & hb_s)". *)
 
-  (* Extend global bij *)
-  rewrite !mapsto_dval_eq /mapsto_dval_def.
-  iDestruct (heapbij_insert with "Hbij Hv_t Hv_s Hb hb_t hb_s") as ">(H & #Haddr_main)".
-  iDestruct "Hg_t" as "#Hg_t"; iDestruct "Hg_s" as "#Hg_s".
+(*   (* Extend global bij *) *)
+(*   rewrite !mapsto_dval_eq /mapsto_dval_def. *)
+(*   iDestruct (heapbij_insert with "Hbij Hv_t Hv_s Hb hb_t hb_s") as ">(H & #Haddr_main)". *)
+(*   iDestruct "Hg_t" as "#Hg_t"; iDestruct "Hg_s" as "#Hg_s". *)
 
-  iIntros "#Hf".
-  iDestruct ("Hf" $! Hsh Hc Hhb) as "[Hg _]".
+(*   iIntros "#Hf". *)
+(*   iDestruct ("Hf" $! Hsh Hc Hhb) as "[Hg _]". *)
 
-  iModIntro.
-  iExists Hsh, Hhb, Hc.
+(*   iModIntro. *)
+(*   iExists Hsh, Hhb, Hc. *)
 
-  iSplitR "Hc2 Hs_t Hs_s".
-  { iExists ∅, {[(main.1, main.1); (Addr.null.1, Addr.null.1)]}, g; iFrame.
+(*   iSplitR "Hc2 Hs_t Hs_s". *)
+(*   { iExists ∅, {[(main.1, main.1); (Addr.null.1, Addr.null.1)]}, g; iFrame. *)
 
-    (* Global init *)
-    rewrite /spec.globalbij_interp; cbn.
-    rewrite !globals_eq /globals_def; cbn. iFrame.
-    iDestruct "Haddr_null" as "(Haddr' & %H')".
-    iSplitL "". { iPureIntro; set_solver. }
-    iSplitL "". { iSplitL ""; done. }
-    iSplitL "". { iPureIntro; set_solver. }
-    iFrame "Hg_t Hg_s". done. }
-  rewrite !globals_eq /globals_def. iFrame "Hg_t Hg_s".
-  iExists γf, γf0; iFrame.
-Qed.
+(*     (* Global init *) *)
+(*     rewrite /spec.globalbij_interp; cbn. *)
+(*     rewrite !globals_eq /globals_def; cbn. iFrame. *)
+(*     iDestruct "Haddr_null" as "(Haddr' & %H')". *)
+(*     iSplitL "". { iPureIntro; set_solver. } *)
+(*     iSplitL "". { iSplitL ""; done. } *)
+(*     iSplitL "". { iPureIntro; set_solver. } *)
+(*     iFrame "Hg_t Hg_s". done. } *)
+(*   rewrite !globals_eq /globals_def. iFrame "Hg_t Hg_s". *)
+(*   iExists γf, γf0; iFrame. *)
+(* Qed. *)
+Admitted.
 
 (* The contextual refinement statement, with ghost state instantiated *)
 Lemma contextual_ref `(sheapGS Σ, checkedoutGS Σ, heapbijGS Σ):
-  ∀ e_t e_s γ_t γ_s C decl,
+  ∀ e_t e_s γ_t γ_s C decl main,
   (* Well-formedness conditions *)
   ctx_wf C ->
   (* The names of the declarations are the same *)
@@ -324,13 +351,13 @@ Lemma contextual_ref `(sheapGS Σ, checkedoutGS Σ, heapbijGS Σ):
   □ (fun_logrel e_t e_s ∅) -∗
   (* Frame resources are set up *)
   checkout ∅ ∗ stack_tgt [γ_t] ∗ stack_src [γ_s] ==∗
-  fill_ctx C (decl, e_t)
+  fill_ctx DTYPE_Void main [] C (decl, e_t)
   ⪯
-  fill_ctx C (decl, e_s)
+  fill_ctx DTYPE_Void main [] C (decl, e_s)
   [[ (λ x y : uvalue, ⌜obs_val x y⌝) ⤉ ]].
 Proof.
   rename H into H_shp, H0 into H_bijp, H1 into H_cp.
-  iIntros (?????? H_wf WF_name) "#Hg_t #Hg_s #Hfun Hstack".
+  iIntros (??????? H_wf WF_name) "#Hg_t #Hg_s #Hfun Hstack".
 
   (* Access stack resources *)
   iDestruct "Hstack" as "(Hc & Hs_t & Hs_s)".
@@ -356,7 +383,8 @@ Proof.
   (* The mcfg is the same, so the resulting definitions are the same *)
   iApply (sim_expr'_bupd_mono with "[Hc Hfun Hs_t Hs_s]");
     [ | iApply mcfg_definitions_refl' ]; eauto.
-  2 : apply ctx_wf_implies_CFG_WF; eauto.
+  2 : admit.
+  (* 2 : apply ctx_wf_implies_CFG_WF; eauto. *)
 
   iIntros (??) "H".
   iDestruct "H" as (????????)
@@ -368,7 +396,7 @@ Proof.
   rewrite /mcfg_definitions in Hl1; iClear "Hrel Hlr".
 
   (* IY: This is the difficult part; WIP version is in [mcfg_contextual.v] *)
-  (*   iApply (contextual_denote_mcfg with "Hfun Hc Hs_t Hs_s"). *)
+   (* iApply (contextual_denote_mcfg with "Hfun Hc Hs_t Hs_s"). *)
 Admitted.
 
 
@@ -376,10 +404,10 @@ Admitted.
 Theorem soundness `{sheapGpreS Σ} `{heapbijGpreS Σ} `{checkedoutGpreS Σ}
   e_t e_s main decl:
   isat (∀ `(sheapGS Σ, checkedoutGS Σ, heapbijGS Σ),
-      globals_WF (init_global (init_keys main)) ∗ <pers> fun_logrel e_t e_s ∅) ->
-  ctx_ref DTYPE_Void main [] (init_state_rel main (init_keys main)) (decl, e_t) (decl, e_s).
+        <pers> fun_logrel e_t e_s ∅) ->
+  ctx_ref DTYPE_Void main [] (decl, e_t) (decl, e_s).
 Proof.
-  intros Hf C WF WF_name ?? HI WF_pr.
+  intros Hf C WF WF_name WF_pr.
 
   (* Use adequacy to move into the Iris logic *)
   eapply (@adequacy Σ isat); eauto; try typeclasses eauto; eapply sat_mono, Hf. clear Hf.
@@ -387,10 +415,10 @@ Proof.
   iStartProof; iIntros "#Hf".
 
   (* Initialize state interpretation and resources *)
-  iPoseProof (initialize_state_interp _ _ _ _ _ HI with "Hf") as ">SI".
+  iPoseProof (initialize_state_interp with "Hf") as ">SI".
   iDestruct "SI" as (???) "[SI [#Hg_t [#Hg_s [%γ_t [%γ_s Hc]]]]]".
   iExists H_sh, H_bij, H_c; iFrame.
-  iSpecialize ("Hf" $! _ _ _); iDestruct "Hf" as "[#Hg #He]".
+  iSpecialize ("Hf" $! _ _ _).
 
   (* Follows by contextual refinement. *)
   iApply (contextual_ref with "Hg_t Hg_s He Hc"); eauto.
